LeanSAT/Data/PPA.lean
@@ -1,11 +1,30 @@
-import Mathlib.Data.Nat.Basic
+/-
+
+Persistent partial assignments and substitutions.
+
+Resizable arrays that can be ``cleared'' in O(1) time by bumping a generation
+number. Each cell in the array stores a generation number that determines if the
+cell is set (i.e. that it is above the data structure's generation number).
+Used to implement partial assignments and substitutions by assuming that all
+variables are unset (PPA) or set to themselves (PS) at initialization.
+
+Authors: Cayden Codel, Wojciech Nawrocki, James Gallicchio
+Carnegie Mellon University
+-/
 
 import LeanSAT.Data.Cnf
 import LeanSAT.Data.ICnf
 import LeanSAT.AuxDefs
 import LeanSAT.Upstream.ToStd
+import LeanSAT.Upstream.ToMathlib
+import Mathlib.Data.Nat.Basic
+import LeanSAT.Model.PropFun
 
 open LeanSAT LeanSAT.Model Nat
+open LitVar ILit IVar LawfulLitVar
+open PropFun
+
+/-! # Concise PPA (single array) -/
 
 /-- A Persistent Partial Assignment of truth values to propositional variables.
 
@@ -28,10 +47,10 @@ structure PPA where
   when the assignment is reset.
   Instead, we just bump the counter and interpret values in the array
   below the counter as unassigned. -/
-  generation : { g : Nat // 0 < g }
+  generation : PNat
   /-- The maximum absolute value of any entry in `assignments`. -/
   maxGen : Nat
-  le_maxGen : ∀ g ∈ assignment.data, g.natAbs ≤ maxGen
+  le_maxGen : ∀ i ∈ assignment.data, i.natAbs ≤ maxGen
 
 instance : ToString PPA where
   toString τ := String.intercalate " ∧ "
@@ -40,33 +59,26 @@ instance : ToString PPA where
 /-! ## Reading values from the PPA -/
 
 namespace PPA
-open LitVar PropFun
 
 @[reducible] def size (τ : PPA) : Nat := τ.assignment.size
 
 def varValue? (τ : PPA) (v : IVar) : Option Bool :=
-  match τ.assignment.get? (v - 1) with
+  match τ.assignment.get? v.index with
   | none => none
   | some n =>
-    if τ.generation.val ≤ n.natAbs then
+    if τ.generation ≤ n.natAbs then
       some (0 < n)
     else
       none
 
-  -- Cayden: Alternative definition that uses a let, not a match:
-  --let v := τ.assignment.getD ((toVar l).val - 1) 0
-  --if τ.generation ≤ v.natAbs then
-  --  some <| xor (v < 0) (polarity l)
-  --else none
-
 /-- The value of the given literal in the current assignment, if assigned.
-Otherwise `none`. -/
+    Otherwise `none`. -/
 def litValue? (τ : PPA) (l : ILit) : Option Bool :=
   τ.varValue? (toVar l) |>.map (fun b => xor (!b) (polarity l))
 
 /-! ### Lemmas about `litValue?`, `varValue?` -/
 
-theorem litValue?_negate (τ : PPA) (l : ILit) :
+@[simp] theorem litValue?_negate (τ : PPA) (l : ILit) :
     τ.litValue? (-l) = (τ.litValue? l).map Bool.not := by
   aesop (add norm unfold litValue?)
 
@@ -78,45 +90,39 @@ theorem litValue?_eq_varValue?_some {τ : PPA} {l : ILit} {b : Bool} :
     τ.litValue? l = some b → τ.varValue? (toVar l) = xor (!b) (polarity l) := by
   aesop (add norm unfold litValue?)
 
-theorem lt_size_of_varValue?_eq_some {τ : PPA} {x : IVar} {b : Bool} :
-    τ.varValue? x = some b → x - 1 < τ.size := by
-  unfold varValue?
-  split
-  . simp
-  next _ _ h =>
-    intros
-    rw [Array.get?_eq_data_get?] at h
-    exact List.get?_eq_some.mp h |>.fst
+theorem lt_size_of_varValue?_eq_some {τ : PPA} {v : IVar} {b : Bool} :
+    τ.varValue? v = some b → v.index < τ.size := by
+  intro hv
+  simp [varValue?, Array.get?] at hv
+  rcases Nat.lt_trichotomy v.index τ.size with (hlt | heq | hgt)
+  · exact hlt
+  · simp [heq] at hv
+  · simp [Nat.lt_asymm hgt] at hv
 
 theorem lt_size_of_litValue?_eq_some {τ : PPA} {l : ILit} {b : Bool} :
-    τ.litValue? l = some b → ((toVar l) - 1) < τ.size := by
-  simp only [litValue?, Option.map_eq_some']
-  intro ⟨b, h⟩
-  exact lt_size_of_varValue?_eq_some h.1
+    τ.litValue? l = some b → (toVar l).index < τ.size := by
+  simp [litValue?]
+  rw [← toVar_index_eq_index]
+  rintro (⟨hv, _⟩ | ⟨hv, _⟩)
+  <;> exact lt_size_of_varValue?_eq_some hv
 
 /-! ### `toPropFun` model -/
 
-def varToPropFun (τ : PPA) (x : IVar) : PropFun IVar :=
-  τ.varValue? x |>.map (if · then .var x else (.var x)ᶜ) |>.getD ⊤
+def varToPropFun (τ : PPA) (v : IVar) : PropFun IVar :=
+  τ.varValue? v |>.map (if · then .var v else (.var v)ᶜ) |>.getD ⊤
 
 def idxToPropFun (τ : PPA) (i : Fin τ.size) : PropFun IVar :=
-  τ.varToPropFun ⟨i + 1, succ_pos _⟩
+  τ.varToPropFun ⟨IVar.fromIndex i, succ_pos _⟩
 
 /-- We model the `PPA` as the conjunction of all its literals.
-Note that we cannot fully model the `PPA` as just one `PropAssignment`
-because those are required to be total. -/
-/- NOTE: Possible alternative models:
-- A `PropSubst` which acts as the identity on all variables not in the PPA.
-  This has a natural notion of semantic entailment: substituting yields ⊤.
-- A finite set of literals. This however doesn't seem to have a natural entailment;
-  there are two, treating the set as either big conj or big disj.
-  Furthermore a set can be inconsistent/tautological
-  by containing complementary literals,
-  and this case has to be handled in such a model,
-  whereas the PPA cannot.
-  The same issue appears with PropFun; see `toPropFun_ne_bot`. -/
+    Note that we cannot fully model the `PPA` as just one `PropAssignment`
+    because those are required to be total. -/
 def toPropFun (τ : PPA) : PropFun IVar :=
   Fin.foldl τ.size (· ⊓ τ.idxToPropFun ·) ⊤
+
+-- Cayden TODO: Having trouble synthesizing the SemanticEntails for IVar from generic ν
+instance : SemanticEntails (PropAssignment IVar) (PropFun IVar) where
+  entails := PropFun.satisfies
 
 theorem satisfies_iff {τ : PPA} {σ : PropAssignment IVar} :
     σ ⊨ τ.toPropFun ↔ ∀ (i : Fin τ.size), σ ⊨ τ.idxToPropFun i := by
@@ -127,20 +133,19 @@ theorem satisfies_iff {τ : PPA} {σ : PropAssignment IVar} :
     simp_all
   . intro h
     unfold toPropFun
-    apply Fin.foldl_induction' (hInit := satisfies_tr)
+    apply Fin.foldl_induction' (hInit := PropFun.satisfies_tr)
     intro ϕ i hϕ
     simp [hϕ, h i]
 
 theorem satisfies_iff_vars {τ : PPA} {σ : PropAssignment IVar} :
-    σ ⊨ τ.toPropFun ↔ ∀ x b, τ.varValue? x = some b → σ x = b := by
+    σ ⊨ τ.toPropFun ↔ ∀ ⦃v⦄ ⦃b⦄, τ.varValue? v = some b → σ v = b := by
   constructor
-  . intro h x b h'
+  . rintro h ⟨v, hv⟩ b h'
     have := lt_size_of_varValue?_eq_some h'
-    let i : Fin τ.size := ⟨Subtype.val x - 1, this⟩
+    let i : Fin τ.size := ⟨v - 1, this⟩
     have h := satisfies_iff.mp h i
     dsimp [idxToPropFun, varToPropFun] at h
-    have : 1 ≤ Subtype.val x := x.property
-    simp_rw [Nat.sub_add_cancel this, Subtype.eta, h'] at h
+    simp_rw [IVar.fromIndex, Nat.sub_add_cancel hv, PNat.val, h'] at h
     simp only [Option.map_some', Option.getD_some] at h
     cases b <;> simp_all
   . intro h
@@ -149,11 +154,11 @@ theorem satisfies_iff_vars {τ : PPA} {σ : PropAssignment IVar} :
     unfold idxToPropFun varToPropFun
     cases' h' : (varValue? τ _) with b
     . simp
-    . have := h _ _ h'
+    . have := h h'
       cases b <;> simp_all
 
 theorem satisfies_iff_lits {τ : PPA} {σ : PropAssignment IVar} :
-    σ ⊨ τ.toPropFun ↔ ∀ l, τ.litValue? l = some true → σ ⊨ LitVar.toPropFun l := by
+    σ ⊨ τ.toPropFun ↔ ∀ ⦃l⦄, τ.litValue? l = some true → σ ⊨ l.toPropFun := by
   simp_rw [LitVar.satisfies_iff, litValue?]
   constructor
   . intro h l h'
@@ -162,8 +167,8 @@ theorem satisfies_iff_lits {τ : PPA} {σ : PropAssignment IVar} :
   . intro h
     apply satisfies_iff_vars.mpr
     intro x b
-    have := h (mkPos x)
-    have := h (mkNeg x)
+    have := @h (mkPos x)
+    have := @h (mkNeg x)
     cases b <;> simp_all
 
 /-- A satisfying assignment for `toPropFun`.
@@ -179,72 +184,70 @@ theorem toPropFun_ne_bot (τ : PPA) : τ.toPropFun ≠ ⊥ := by
   have := τ.toSatAssignment_satisfies
   simp_all only [not_satisfies_fls]
 
-theorem varValue?_true (τ : PPA) (x : IVar) :
-    τ.varValue? x = some true → τ.toPropFun ≤ .var x := by
+theorem varValue?_true {τ : PPA} {v : IVar} :
+    τ.varValue? v = some true → τ.toPropFun ≤ .var v := by
   intro h
   apply PropFun.entails_ext.mpr
   simp_all [satisfies_iff_vars]
 
-theorem varValue?_false (τ : PPA) (x : IVar) :
-    τ.varValue? x = some false → τ.toPropFun ≤ (.var x)ᶜ := by
+theorem varValue?_false {τ : PPA} {v : IVar} :
+    τ.varValue? v = some false → τ.toPropFun ≤ (.var v)ᶜ := by
   intro h
   apply PropFun.entails_ext.mpr
   simp_all [satisfies_iff_vars]
 
-theorem not_mem_semVars_of_varValue?_none (τ : PPA) (x : IVar) :
-    τ.varValue? x = none → x ∉ τ.toPropFun.semVars := by
+theorem not_mem_semVars_of_varValue?_none {τ : PPA} {v : IVar} :
+    τ.varValue? v = none → v ∉ τ.toPropFun.semVars := by
   rw [not_mem_semVars]
-  intro hx σ b hσ
+  intro hv σ b hσ
   rw [satisfies_iff_vars] at hσ ⊢
   intro y b hy
-  have : x ≠ y := fun h => by rw [h, hy] at hx; contradiction
+  have : v ≠ y := fun h => by rw [h, hy] at hv; contradiction
   rw [PropAssignment.set_get_of_ne _ _ this]
-  apply hσ y b hy
+  apply hσ hy
 
-theorem varValue?_none (τ : PPA) (x : IVar) :
-    τ.varValue? x = none → ¬(τ.toPropFun ≤ .var x) := by
+theorem varValue?_none {τ : PPA} {v : IVar} :
+    τ.varValue? v = none → ¬(τ.toPropFun ≤ .var v) := by
   intro hNone hLt
-  let σ := τ.toSatAssignment.set x false
+  let σ := τ.toSatAssignment.set v false
   have : σ.agreeOn τ.toPropFun.semVars τ.toSatAssignment := fun y hMem =>
-    have : x ≠ y := fun h => τ.not_mem_semVars_of_varValue?_none x hNone (h ▸ hMem)
+    have : v ≠ y := fun h => τ.not_mem_semVars_of_varValue?_none hNone (h ▸ hMem)
     PropAssignment.set_get_of_ne _ _ this
   have hσ : σ ⊨ τ.toPropFun := (agreeOn_semVars this).mpr τ.toSatAssignment_satisfies
-  have : σ ⊭ .var x := by
+  have : σ ⊭ .var v := by
     simp only [satisfies_var, PropAssignment.set_get, not_false_eq_true]
   exact this (entails_ext.mp hLt σ hσ)
 
-theorem varValue?_none' (τ : PPA) (x : IVar) :
-    τ.varValue? x = none → ¬(τ.toPropFun ≤ (.var x)ᶜ) := by
+theorem varValue?_none' {τ : PPA} {v : IVar} :
+    τ.varValue? v = none → ¬(τ.toPropFun ≤ (.var v)ᶜ) := by
   intro hNone hLt
-  let σ := τ.toSatAssignment.set x true
+  let σ := τ.toSatAssignment.set v true
   have : σ.agreeOn τ.toPropFun.semVars τ.toSatAssignment := fun y hMem =>
-    have : x ≠ y := fun h => τ.not_mem_semVars_of_varValue?_none x hNone (h ▸ hMem)
+    have : v ≠ y := fun h => τ.not_mem_semVars_of_varValue?_none hNone (h ▸ hMem)
     PropAssignment.set_get_of_ne _ _ this
   have hσ : σ ⊨ τ.toPropFun := (agreeOn_semVars this).mpr τ.toSatAssignment_satisfies
-  have : σ ⊭ (.var x)ᶜ := by
+  have : σ ⊭ (.var v)ᶜ := by
     simp only [PropFun.satisfies_neg, satisfies_var, PropAssignment.set_get, not_true_eq_false,
       not_false_eq_true]
   exact this (entails_ext.mp hLt σ hσ)
 
-theorem litValue?_true (τ : PPA) (l : ILit) :
-    τ.litValue? l = some true → τ.toPropFun ≤ LitVar.toPropFun l := by
+theorem litValue?_true {τ : PPA} {l : ILit} :
+    τ.litValue? l = some true → τ.toPropFun ≤ l.toPropFun := by
   simp [litValue?, LitVar.toPropFun]
   cases polarity l <;>
     simp (config := {contextual := true}) [varValue?_false, varValue?_true]
 
-theorem litValue?_false (τ : PPA) (l : ILit) :
-    τ.litValue? l = some false → τ.toPropFun ≤ (LitVar.toPropFun l)ᶜ := by
+theorem litValue?_false {τ : PPA} {l : ILit} :
+    τ.litValue? l = some false → τ.toPropFun ≤ (l.toPropFun)ᶜ := by
   simp [litValue?, LitVar.toPropFun]
   cases polarity l <;>
     simp (config := {contextual := true}) [varValue?_false, varValue?_true]
 
-theorem litValue?_none (τ : PPA) (l : ILit) :
-    τ.litValue? l = none → ¬(τ.toPropFun ≤ LitVar.toPropFun l) := by
+theorem litValue?_none {τ : PPA} {l : ILit} :
+    τ.litValue? l = none → ¬(τ.toPropFun ≤ l.toPropFun) := by
   simp [litValue?, LitVar.toPropFun]
   cases (polarity l) <;>
     simp (config := {contextual := true}) [varValue?_none, varValue?_none']
-
-end PPA
 
 -- ?? folded into the `PPA` structure for now (forever?)
 --structure PPA.WF (ppa : PPA) where
@@ -253,32 +256,29 @@ end PPA
 
 /-! ## Setting values in the PPA -/
 
-namespace PPA
-  open LitVar PropFun
+/-- Initialize to an empty partial assignment,
+supporting variables in the range `[1, maxVar]`.
 
-  /-- Initialize to an empty partial assignment,
-  supporting variables in the range `[1, maxVar]`.
+The assignment will resize dynamically if it's used with
+a variable above the initial `maxVar`. -/
+def new (maxVar : Nat) : PPA where
+  assignment := Array.mkArray maxVar 0
+  generation := ⟨1, Nat.one_pos⟩
+  maxGen := 0
+  le_maxGen i h := by simp_all [List.mem_replicate]
 
-  The assignment will resize dynamically if it's used with
-  a variable above the initial `maxVar`. -/
-  def new (maxVar : Nat) : PPA where
-    assignment := Array.mkArray maxVar 0
-    generation := ⟨1, Nat.one_pos⟩
-    maxGen := 0
-    le_maxGen i h := by simp_all [List.mem_replicate]
+/-- Reset the assignment to an empty one. -/
+def reset (τ : PPA) : PPA :=
+  { τ with generation := ⟨τ.maxGen + 1, Nat.succ_pos _⟩ }
 
-  /-- Reset the assignment to an empty one. -/
-  def reset (τ : PPA) : PPA :=
-    { τ with generation := ⟨τ.maxGen + 1, Nat.succ_pos _⟩ }
+/-- Clear all temporary assignments at the current generation. -/
+def bump (τ : PPA) : PPA :=
+  { τ with generation := ⟨τ.generation + 1, Nat.succ_pos _⟩ }
 
-  /-- Clear all temporary assignments at the current generation. -/
-  def bump (τ : PPA) : PPA :=
-    { τ with generation := ⟨τ.generation + 1, Nat.succ_pos _⟩ }
-
-  /-- Helper theorem for `setVar*`. -/
-  theorem setVar_le_maxGen (τ : PPA) (i : Nat) (b : Bool) (gen : Nat) :
-    let v : Int := if b then gen else -gen
-    ∀ g ∈ (τ.assignment.setF i v 0).data, g.natAbs ≤ Nat.max τ.maxGen gen := by
+/-- Helper theorem for `setVar*`. -/
+theorem setVar_le_maxGen (τ : PPA) (i : Nat) (b : Bool) (gen : Nat) :
+  let v : Int := if b then gen else -gen
+  ∀ g ∈ (τ.assignment.setF i v 0).data, g.natAbs ≤ Nat.max τ.maxGen gen := by
   intro v g hg
   have := Array.mem_setF _ _ _ _ g hg
   rcases this with h | h | h
@@ -286,339 +286,513 @@ namespace PPA
   . simp [h]
   . cases b <;> simp [h]
 
-  /-- Set the given variable to `b` for the current generation. -/
-  def setVar (τ : PPA) (x : IVar) (b : Bool) : PPA :=
-    let v : Int := if b then τ.generation else -τ.generation
-    { τ with
-      assignment := τ.assignment.setF (x - 1) v 0
-      maxGen := Nat.max τ.maxGen τ.generation
-      le_maxGen := setVar_le_maxGen τ (x - 1) b τ.generation
-    }
+/-- Set the given variable to `b` for the current generation. -/
+def setVar (τ : PPA) (v : IVar) (b : Bool) : PPA :=
+  let g : Int := if b then τ.generation else -τ.generation
+  { τ with
+    assignment := τ.assignment.setF v.index g 0
+    maxGen := Nat.max τ.maxGen τ.generation
+    le_maxGen := setVar_le_maxGen τ v.index b τ.generation }
 
-  /-- Set the given literal to `true` for the current generation. -/
-  def setLit (τ : PPA) (l : ILit) : PPA :=
-    τ.setVar (toVar l) (polarity l)
+/-- Set the given literal to `true` for the current generation. -/
+def setLit (τ : PPA) (l : ILit) : PPA :=
+  τ.setVar (toVar l) (polarity l)
 
-  /-- Set the given variable to `b` for all generations until `gen`. -/
-  def setVarUntil (τ : PPA) (x : IVar) (b : Bool) (gen : Nat) : PPA :=
-    let v : Int := if b then gen else -gen
-    { τ with
-      assignment := τ.assignment.setF (x - 1) v 0
-      maxGen := Nat.max τ.maxGen gen
-      le_maxGen := setVar_le_maxGen τ (x - 1) b gen
-    }
+/-- Set the given variable to `b` for all generations until `gen`. -/
+def setVarUntil (τ : PPA) (v : IVar) (b : Bool) (gen : Nat) : PPA :=
+  let g : Int := if b then gen else -gen
+  { τ with
+    assignment := τ.assignment.setF v.index g 0
+    maxGen := Nat.max τ.maxGen gen
+    le_maxGen := setVar_le_maxGen τ v.index b gen }
 
-  /-- Set the given literal to `true` for all generations until `gen`. -/
-  def setLitUntil (τ : PPA) (l : ILit) (gen : Nat) : PPA :=
-    τ.setVarUntil (toVar l) (polarity l) gen
+/-- Set the given literal to `true` for all generations until `gen`. -/
+def setLitUntil (τ : PPA) (l : ILit) (gen : Nat) : PPA :=
+  τ.setVarUntil (toVar l) (polarity l) gen
 
-  /-- Set `l ↦ ⊥` for each `l ∈ C` and leave the rest of the assignment untouched.
-  If the current assignment contains literals appearing in `C`, they will be overwritten. -/
-  def setNegatedClause (τ : PPA) (C : IClause) : PPA :=
-    C.foldl (init := τ) (fun τ l => τ.setLit (-l))
+/-- Set `l ↦ ⊥` for each `l ∈ C` and leave the rest of the assignment untouched.
+If the current assignment contains literals appearing in `C`, they will be overwritten. -/
+def setNegatedClause (τ : PPA) (C : IClause) : PPA :=
+  C.foldl (init := τ) (fun τ l => τ.setLit (-l))
 
-  def setNegatedClauseUntil (τ : PPA) (C : IClause) (gen : Nat) : PPA :=
-    C.foldl (init := τ) (fun τ l => τ.setLitUntil (-l) gen)
+def setNegatedClauseUntil (τ : PPA) (C : IClause) (gen : Nat) : PPA :=
+  C.foldl (init := τ) (fun τ l => τ.setLitUntil (-l) gen)
 
-  /-! ### Lemmas about `reset` -/
+/-! ### Lemmas about `reset` -/
 
-  theorem lt_reset_generation (τ : PPA) : ∀ i ∈ τ.reset.assignment.data, i.natAbs < τ.reset.generation := by
-    dsimp [reset]
-    intro i h
-    have := τ.le_maxGen i h
-    linarith
+theorem lt_reset_generation (τ : PPA) : ∀ i ∈ τ.reset.assignment.data, i.natAbs < τ.reset.generation := by
+  dsimp [reset]
+  intro i h
+  have := τ.le_maxGen i h
+  linarith
 
-  @[simp]
-  theorem varValue?_reset (τ : PPA) (x : IVar) : τ.reset.varValue? x = none := by
-    unfold varValue?
-    split
+@[simp]
+theorem varValue?_reset (τ : PPA) (v : IVar) : τ.reset.varValue? v = none := by
+  unfold varValue?
+  split
+  . rfl
+  . split
+    . next n hn h =>
+      have : n ∈ τ.reset.assignment.data := by
+        simp_rw [Array.get?_eq_getElem?, Array.getElem?_eq_data_get?, List.get?_eq_some] at hn
+        have ⟨_, hn⟩ := hn
+        rw [← hn]
+        apply List.get_mem
+      have := τ.lt_reset_generation n this
+      linarith
     . rfl
-    . split
-      . next n hn h =>
-        have : n ∈ τ.reset.assignment.data := by
-          simp_rw [Array.get?_eq_getElem?, Array.getElem?_eq_data_get?, List.get?_eq_some] at hn
-          have ⟨_, hn⟩ := hn
-          rw [← hn]
-          apply List.get_mem
-        have := τ.lt_reset_generation n this
-        linarith
-      . rfl
 
-  @[simp]
-  theorem litValue?_reset (τ : PPA) (l : ILit) : (τ.reset).litValue? l = none := by
-    simp [litValue?, varValue?_reset]
+@[simp]
+theorem litValue?_reset (τ : PPA) (l : ILit) : (τ.reset).litValue? l = none := by
+  simp [litValue?, varValue?_reset]
 
-  @[simp]
-  theorem toPropFun_reset (τ : PPA) : τ.reset.toPropFun = ⊤ := by
-    ext; simp [satisfies_iff_vars]
+@[simp]
+theorem toPropFun_reset (τ : PPA) : τ.reset.toPropFun = ⊤ := by
+  ext; simp [satisfies_iff_vars]
 
-  /-! ### Lemmas about `setVar`, `setLit` -/
+/-! ### Lemmas about `setVar`, `setLit` -/
 
-  @[simp]
-  theorem varValue?_setVar (τ : PPA) (x : IVar) (b : Bool) : (τ.setVar x b).varValue? x = some b := by
-    unfold varValue? setVar
-    cases b <;> simp [Array.getElem?_setF, τ.generation.property]
+@[simp]
+theorem varValue?_setVar (τ : PPA) (v : IVar) (b : Bool) : (τ.setVar v b).varValue? v = some b := by
+  unfold varValue? setVar
+  cases b <;> simp [Array.getElem?_setF, τ.generation.property]
 
-  @[simp]
-  theorem varValue?_setVar_of_ne (τ : PPA) {x x' : IVar} (b : Bool) :
-      x ≠ x' → (τ.setVar x b).varValue? x' = τ.varValue? x' := by
-    unfold varValue? setVar
-    intro hNe
-    have : x.val - 1 ≠ x'.val - 1 := by
+@[simp]
+theorem varValue?_setVar_of_ne {v v' : IVar} :
+    v ≠ v' → ∀ (τ : PPA) (b : Bool), (τ.setVar v b).varValue? v' = τ.varValue? v' := by
+  unfold varValue? setVar
+  intro hNe
+  simp [Array.getElem?_setF' _ _ _ (index_ne_iff.mpr hNe)]
+
+@[simp]
+theorem varValue?_setLit (τ : PPA) (l : ILit) : (τ.setLit l).varValue? (toVar l) = some (polarity l) := by
+  simp [setLit, varValue?_setVar]
+
+@[simp]
+theorem litValue?_setLit (τ : PPA) (l : ILit) : (τ.setLit l).litValue? l = some true := by
+  simp [litValue?, setLit, varValue?_setVar]
+
+@[simp]
+theorem varValue?_setLit_of_ne {l : ILit} {v : IVar} :
+    toVar l ≠ v → ∀ (τ : PPA), (τ.setLit l).varValue? v = τ.varValue? v := by
+  intro h
+  simp [setLit, varValue?_setVar_of_ne h]
+
+@[simp]
+theorem litValue?_setLit_of_ne {l l' : ILit} :
+    toVar l ≠ toVar l' → ∀ (τ : PPA), (τ.setLit l).litValue? l' = τ.litValue? l' := by
+  intro h
+  simp [litValue?, varValue?_setLit_of_ne h]
+
+/-! ### `toPropFun` model -/
+
+theorem toPropFun_setVar_lt_of_none {τ : PPA} {v : IVar} :
+    τ.varValue? v = none → ∀ (b : Bool), (τ.setVar v b).toPropFun ≤ τ.toPropFun := by
+  intro h b
+  apply entails_ext.mpr
+  intro σ hσ
+  rw [satisfies_iff_vars] at hσ ⊢
+  intro y b hy
+  apply hσ
+  rwa [varValue?_setVar_of_ne]
+  intro hEq
+  rw [hEq, hy] at h
+  contradiction
+
+theorem toPropFun_setLit_lt_of_none {τ : PPA} {l : ILit} :
+    τ.litValue? l = none → (τ.setLit l).toPropFun ≤ τ.toPropFun := by
+  intro
+  simp_all only [litValue?, setLit, Option.map_eq_none', toPropFun_setVar_lt_of_none]
+
+theorem toPropFun_setLit_lt (τ : PPA) (l : ILit) :
+    (τ.setLit l).toPropFun ≤ l.toPropFun := by
+  apply entails_ext.mpr
+  intro σ hσ
+  rw [satisfies_iff_lits] at hσ
+  apply hσ
+  apply litValue?_setLit
+
+theorem lt_toPropFun_setLit (τ : PPA) (l : ILit) :
+    τ.toPropFun ⊓ l.toPropFun ≤ (τ.setLit l).toPropFun := by
+  apply entails_ext.mpr
+  intro σ hσ
+  have ⟨hσ, hσ'⟩ := satisfies_conj.mp hσ
+  rw [satisfies_iff_vars] at hσ ⊢
+  intro x b hx
+  by_cases h : toVar l = x
+  . simp_all [setLit, LitVar.satisfies_iff]
+  . apply hσ
+    rwa [τ.varValue?_setLit_of_ne h] at hx
+
+theorem toPropFun_setLit_of_none {τ : PPA} {l : ILit} :
+    τ.litValue? l = none → (τ.setLit l).toPropFun = τ.toPropFun ⊓ l.toPropFun := by
+  intro h
+  refine le_antisymm ?_ (τ.lt_toPropFun_setLit l)
+  simp [toPropFun_setLit_lt_of_none h, toPropFun_setLit_lt]
+
+/-! ## Tautology checking -/
+
+/-- Check if the given clause is a tautology.
+The current partial assignment is ignored,
+and the returned assignment is unspecified. -/
+def checkTauto (τ : PPA) (C : IClause) : PPA × { b : Bool // b ↔ C.toPropFun = ⊤ } :=
+  go 0 ⟨τ.reset, by simp [Clause.toPropFun]⟩
+where
+  go (i : Nat) (τ : { τ : PPA // τ.toPropFunᶜ = Clause.toPropFun ⟨C.data.take i⟩ })
+    : PPA × { b : Bool // b ↔ C.toPropFun = ⊤ } :=
+  if hLt : i < C.size then
+    let l := C[i]'hLt
+    have hCl : Clause.toPropFun ⟨C.data.take (i+1)⟩ = Clause.toPropFun ⟨C.data.take i⟩ ⊔ l.toPropFun := by
+      simp [List.take_succ, List.get?_eq_get hLt, Array.getElem_eq_data_get]
+    match h : τ.val.litValue? l with
+    | some true =>
+      (τ.val, ⟨true, by
+        have : τ.val.toPropFun ≤ l.toPropFun := τ.val.litValue?_true h
+        have : (l.toPropFun)ᶜ ≤ τ.val.toPropFunᶜ := compl_le_compl this
+        have : (l.toPropFun)ᶜ ≤ C.toPropFun := by
+          apply le_trans this
+          rw [τ.property]
+          apply C.toPropFun_take_lt
+        have : l.toPropFun ≤ C.toPropFun := C.toPropFun_getElem_lt i _
+        have : ⊤ ≤ C.toPropFun := by
+          rw [← sup_compl_eq_top (x := l.toPropFun)]
+          apply sup_le <;> assumption
+        simp only [top_le_iff.mp this]⟩)
+    | some false =>
+      go (i + 1) ⟨τ.val.setLit (-l), by
+        have : (τ.val.setLit (-l)).toPropFun ≤ τ.val.toPropFun := by
+          apply entails_ext.mpr
+          intro σ hσ
+          rw [satisfies_iff_vars] at hσ ⊢
+          intro x b hx
+          apply hσ
+          by_cases hEq : toVar (-l) = x
+          . aesop (add norm unfold litValue?, norm unfold setLit)
+          . rwa [τ.val.varValue?_setLit_of_ne hEq]
+        have := τ.val.toPropFun_setLit_lt (-l)
+        have : (τ.val.setLit (-l)).toPropFun = τ.val.toPropFun ⊓ (-l).toPropFun := by
+          refine le_antisymm ?_ (τ.val.lt_toPropFun_setLit _)
+          simp_all only [le_inf_iff, and_self]
+        simp [*, τ.property]⟩
+    | none =>
+      go (i + 1) ⟨τ.val.setLit (-l), by
+        have : (τ.val.setLit (-l)).toPropFun = τ.val.toPropFun ⊓ (-l).toPropFun := by
+          apply toPropFun_setLit_of_none
+          simp [τ.val.litValue?_negate l, h]
+        simp [*, τ.property]⟩
+  else
+    (τ.val, ⟨false, by
+      simp only [false_iff]
       intro h
-      have hx : 1 ≤ x.val := by cases x; assumption
-      have hx' : 1 ≤ x'.val := by cases x'; assumption
-      have : x.val - 1 + 1 = x'.val - 1 + 1 := by simp_rw [h]
-      rw [Nat.sub_add_cancel hx, Nat.sub_add_cancel hx'] at this
-      exact hNe (PNat.coe_inj.mp this)
-    simp [Array.getElem?_setF' _ _ _ this]
+      apply τ.val.toPropFun_ne_bot
+      have hEq := τ.property
+      have : C.data.length ≤ i := by rw [not_lt] at hLt; exact hLt
+      have that : C = { data := C.data } := rfl
+      simp_rw [C.data.take_length_le this, ← that, h, compl_eq_top] at hEq
+      assumption⟩)
+termination_by go i τ => C.size - i
 
-  @[simp]
-  theorem varValue?_setLit (τ : PPA) (l : ILit) : (τ.setLit l).varValue? (toVar l) = some (polarity l) := by
-    simp [setLit, varValue?_setVar]
+/-! ## Unit propagation -/
 
-  @[simp]
-  theorem litValue?_setLit (τ : PPA) (l : ILit) : (τ.setLit l).litValue? l = some true := by
-    simp [litValue?, setLit, varValue?_setVar]
+-- Cayden's alternate formulation of | extended
+-- | extended      (l : ILit)
+--                (τ' : PPA)
+--                (h₁ : C.toPropFun ⊓ τ.toPropFun = τ'.toPropFun)
+--                (h₂ : τ.litValue? l = none ∧ τ'.litValue? l = some true)
 
-  @[simp]
-  theorem varValue?_setLit_of_ne (τ : PPA) (l : ILit) (x : IVar) :
-      toVar l ≠ x → (τ.setLit l).varValue? x = τ.varValue? x := by
-    intro h
-    simp [setLit, varValue?_setVar_of_ne _ _ h]
+inductive UPResult (τ τ' : PPA) (C : IClause) where
+  | contradiction (h : C.toPropFun ⊓ τ.toPropFun = ⊥)
+  /-- Under `τ`, `C` became a unit clause `[l]`.
+  The assignment was extended by that literal, i.e., `τ' = τ ⊓ l`. -/
+  -- Note: I didn't prove that `C' = [l]`.
+  | extended      (l : ILit) (hl : l ∈ C.data)
+                  (h₁ : τ'.toPropFun = l.toPropFun ⊓ τ.toPropFun)
+                  (h₂ : τ.toPropFun ⊓ C.toPropFun ≤ l.toPropFun)
+  /-- Clause became satisfied. -/
+  | satisfied
+  /-- Clause did not become unit, and was not satisfied. -/
+  | notUnit
 
-  @[simp]
-  theorem litValue?_setLit_of_ne (τ : PPA) (l l' : ILit) :
-      toVar l ≠ toVar l' → (τ.setLit l).litValue? l' = τ.litValue? l' := by
-    intro h
-    simp [litValue?, varValue?_setLit_of_ne _ _ _ h]
-
-  /-! ### `toPropFun` model -/
-
-  theorem toPropFun_setVar_lt_of_none (τ : PPA) (x : IVar) (b : Bool) :
-      τ.varValue? x = none → (τ.setVar x b).toPropFun ≤ τ.toPropFun := by
-    intro h
-    apply entails_ext.mpr
-    intro σ hσ
-    rw [satisfies_iff_vars] at hσ ⊢
-    intro y b hy
-    apply hσ
-    rwa [varValue?_setVar_of_ne]
-    intro hEq
-    rw [hEq, hy] at h
-    contradiction
-
-  theorem toPropFun_setLit_lt_of_none (τ : PPA) (l : ILit) :
-      τ.litValue? l = none → (τ.setLit l).toPropFun ≤ τ.toPropFun := by
-    intro
-    simp_all only [litValue?, setLit, Option.map_eq_none', toPropFun_setVar_lt_of_none]
-
-  theorem toPropFun_setLit_lt (τ : PPA) (l : ILit) :
-      (τ.setLit l).toPropFun ≤ LitVar.toPropFun l := by
-    apply entails_ext.mpr
-    intro σ hσ
-    rw [satisfies_iff_lits] at hσ
-    apply hσ
-    apply litValue?_setLit
-
-  theorem lt_toPropFun_setLit (τ : PPA) (l : ILit) :
-      τ.toPropFun ⊓ LitVar.toPropFun l ≤ (τ.setLit l).toPropFun := by
-    apply entails_ext.mpr
-    intro σ hσ
-    have ⟨hσ, hσ'⟩ := satisfies_conj.mp hσ
-    rw [satisfies_iff_vars] at hσ ⊢
-    intro x b hx
-    by_cases h : toVar l = x
-    . simp_all [setLit, LitVar.satisfies_iff]
-    . apply hσ
-      rwa [τ.varValue?_setLit_of_ne _ _ h] at hx
-
-  theorem toPropFun_setLit_of_none (τ : PPA) (l : ILit) :
-      τ.litValue? l = none → (τ.setLit l).toPropFun = τ.toPropFun ⊓ LitVar.toPropFun l := by
-    intro h
-    refine le_antisymm ?_ (τ.lt_toPropFun_setLit l)
-    simp [toPropFun_setLit_lt_of_none _ _ h, toPropFun_setLit_lt]
-
-  /-! ## Lemmas about `setNegatedClause` -/
-
-  @[simp]
-  theorem toPropFun_reset_setNegatedClause (τ : PPA) (C : IClause) :
-      -- NOTE: We only get an equality if `C.toPropFun ≠ ⊤`.
-      C.toPropFunᶜ ≤ (τ.reset.setNegatedClause C).toPropFun := by
-    suffices (Clause.toPropFun { data := C.data.take C.size : IClause })ᶜ ≤ (τ.reset.setNegatedClause C).toPropFun by
-      simpa using this
-    unfold setNegatedClause
-    apply Array.foldl_induction
-      (motive := fun n acc => (Clause.toPropFun { data := C.data.take n : IClause })ᶜ ≤ PPA.toPropFun acc)
-    . simp [Clause.toPropFun]
-    . intro i τ ih
-      refine le_trans (le_inf_iff.mpr ?_) (τ.lt_toPropFun_setLit (-C[i]))
-      simp only [List.take_succ, Clause.of_append, Clause.toPropFun_append, compl_sup]
-      constructor
-      . exact inf_le_of_left_le ih
-      . apply inf_le_of_right_le
-        simp [List.get?_eq_get, Array.getElem_eq_data_get]
-
-  /-! ## Tautology checking -/
-
-  /-- Check if the given clause is a tautology.
-  The current partial assignment is ignored,
-  and the returned assignment is unspecified. -/
-  def checkTauto (τ : PPA) (C : IClause) : PPA × { b : Bool // b ↔ C.toPropFun = ⊤ } :=
-    go 0 ⟨τ.reset, by simp [Clause.toPropFun]⟩
-  where
-    go (i : Nat) (τ : { τ : PPA // τ.toPropFunᶜ = Clause.toPropFun ⟨C.data.take i⟩ })
-      : PPA × { b : Bool // b ↔ C.toPropFun = ⊤ } :=
-    if hLt : i < C.size then
-      let l := C[i]'hLt
-      have hCl : Clause.toPropFun ⟨C.data.take (i+1)⟩ = Clause.toPropFun ⟨C.data.take i⟩ ⊔ LitVar.toPropFun l := by
-        simp [List.take_succ, List.get?_eq_get hLt, Array.getElem_eq_data_get]
-      match h : τ.val.litValue? l with
-      | some true =>
-        (τ.val, ⟨true, by
-          have : τ.val.toPropFun ≤ LitVar.toPropFun l := τ.val.litValue?_true l h
-          have : (LitVar.toPropFun l)ᶜ ≤ τ.val.toPropFunᶜ := compl_le_compl this
-          have : (LitVar.toPropFun l)ᶜ ≤ C.toPropFun := by
-            apply le_trans this
-            rw [τ.property]
-            apply C.toPropFun_take_lt
-          have : LitVar.toPropFun l ≤ C.toPropFun := C.toPropFun_getElem_lt i _
-          have : ⊤ ≤ C.toPropFun := by
-            rw [← sup_compl_eq_top (x := LitVar.toPropFun l)]
-            apply sup_le <;> assumption
-          simp only [top_le_iff.mp this]⟩)
+/-- If `C` is satisfied by `τ`, return `satisfied`.
+Otherwise compute the reduced clause `C' = {l ∈ C | ¬l ∉ τ}`.
+If `C' = [u]` is a unit, extend `τ` by `u` and return `extended`.
+If `C'` has become empty (is falsified), return `contradiction`.
+If `C'` is not a unit and not falsified, return `notUnit`. -/
+def propagateUnit (τ : PPA) (C : IClause) : (τ' : PPA) × UPResult τ τ' C :=
+  go 0 none Option.all_none (by simp only [not_lt_zero', IsEmpty.forall_iff, implies_true])
+where
+  /-- If `unit? = some u`, then `u` is a literal in the clause that is not falsified by `τ`.
+  It may therefore be the case that `C' = [u]` -/
+  go (i : Nat) (unit? : Option ILit) (hUnit : unit?.all fun u => u ∈ C.data ∧ τ.litValue? u = none)
+      (hLits : ∀ (j : Fin C.size), j.val < i → unit? = some C[j] ∨ τ.toPropFun ≤ (C[j].toPropFun)ᶜ) :
+      (τ' : PPA) × UPResult τ τ' C :=
+    if hi : i < C.size then
+      let l := C[i]'hi
+      match hl : τ.litValue? l with
+      | some true => ⟨τ, .satisfied⟩
       | some false =>
-        go (i + 1) ⟨τ.val.setLit (-l), by
-          have : (τ.val.setLit (-l)).toPropFun ≤ τ.val.toPropFun := by
-            apply entails_ext.mpr
-            intro σ hσ
-            rw [satisfies_iff_vars] at hσ ⊢
-            intro x b hx
-            apply hσ
-            by_cases hEq : toVar (-l) = x
-            . aesop (add norm unfold litValue?, norm unfold setLit)
-            . rwa [τ.val.varValue?_setLit_of_ne _ _ hEq]
-          have := τ.val.toPropFun_setLit_lt (-l)
-          have : (τ.val.setLit (-l)).toPropFun = τ.val.toPropFun ⊓ LitVar.toPropFun (-l) := by
-            refine le_antisymm ?_ (τ.val.lt_toPropFun_setLit _)
-            simp_all only [le_inf_iff, and_self]
-          simp [*, τ.property]⟩
+        -- TODO: lots of duplication here
+        go (i+1) unit? hUnit (by
+          intro j hj
+          rcases Nat.lt_or_eq_of_le (Nat.lt_succ.mp hj) with hj | hj
+          . exact hLits j hj
+          . apply Or.inr
+            apply litValue?_false
+            simp [hj, hl])
       | none =>
-        go (i + 1) ⟨τ.val.setLit (-l), by
-          have : (τ.val.setLit (-l)).toPropFun = τ.val.toPropFun ⊓ LitVar.toPropFun (-l) := by
-            apply toPropFun_setLit_of_none
-            simp [τ.val.litValue?_negate l, h]
-          simp [*, τ.property]⟩
-    else
-      (τ.val, ⟨false, by
-        simp only [false_iff]
-        intro h
-        apply τ.val.toPropFun_ne_bot
-        have hEq := τ.property
-        have : C.data.length ≤ i := by rw [not_lt] at hLt; exact hLt
-        have that : C = { data := C.data } := rfl
-        simp_rw [C.data.take_length_le this, ← that, h, compl_eq_top] at hEq
-        assumption⟩)
-  termination_by go i τ => C.size - i
-
-  /-! ## Unit propagation -/
-
-  inductive UPResult (τ τ' : PPA) (C : IClause) where
-    | contradiction (h : C.toPropFun ⊓ τ.toPropFun = ⊥)
-    /-- Under `τ`, `C` became a unit clause `[l]`.
-    The assignment was extended by that literal, i.e., `τ' = τ ⊓ l`. -/
-    -- Note: I didn't prove that `C' = [l]`.
-    | extended      (l : ILit) (hl : l ∈ C.data)
-                    (h₁ : τ'.toPropFun = LitVar.toPropFun l ⊓ τ.toPropFun)
-                    (h₂ : τ.toPropFun ⊓ C.toPropFun ≤ LitVar.toPropFun l)
-    /-- Clause became satisfied. -/
-    | satisfied
-    /-- Clause did not become unit, and was not satisfied. -/
-    | notUnit
-
-  /-- If `C` is satisfied by `τ`, return `satisfied`.
-  Otherwise compute the reduced clause `C' = {l ∈ C | ¬l ∉ τ}`.
-  If `C' = [u]` is a unit, extend `τ` by `u` and return `extended`.
-  If `C'` has become empty (is falsified), return `contradiction`.
-  If `C'` is not a unit and not falsified, return `notUnit`. -/
-  def propagateUnit (τ : PPA) (C : IClause) : (τ' : PPA) × UPResult τ τ' C :=
-    go 0 none Option.all_none (by simp only [not_lt_zero', IsEmpty.forall_iff, implies_true])
-  where
-    /-- If `unit? = some u`, then `u` is a literal in the clause that is not falsified by `τ`.
-    It may therefore be the case that `C' = [u]` -/
-    go (i : Nat) (unit? : Option ILit) (hUnit : unit?.all fun u => u ∈ C.data ∧ τ.litValue? u = none)
-        (hLits : ∀ (j : Fin C.size), j.val < i → unit? = some C[j] ∨ τ.toPropFun ≤ (LitVar.toPropFun C[j])ᶜ) :
-        (τ' : PPA) × UPResult τ τ' C :=
-      if hi : i < C.size then
-        let l := C[i]'hi
-        match hl : τ.litValue? l with
-        | some true => ⟨τ, .satisfied⟩
-        | some false =>
-          -- TODO: lots of duplication here
-          go (i+1) unit? hUnit (by
-            intro j hj
-            rcases Nat.lt_or_eq_of_le (Nat.lt_succ.mp hj) with hj | hj
-            . exact hLits j hj
-            . apply Or.inr
-              apply litValue?_false
-              simp [hj, hl])
-        | none =>
-          match hUnit : unit? with
-          | .some u =>
-            if hEq : u = l then
-              go (i+1) (some l) (by simp [C.getElem_mem_data hi, hl]) (by
-                intro j hj
-                rcases Nat.lt_or_eq_of_le (Nat.lt_succ.mp hj) with hj | hj
-                . exact hEq ▸ hLits j hj
-                . apply Or.inl
-                  simp [hEq, hj])
-            else
-              ⟨τ, .notUnit⟩
-          | .none =>
+        match hUnit : unit? with
+        | .some u =>
+          if hEq : u = l then
             go (i+1) (some l) (by simp [C.getElem_mem_data hi, hl]) (by
               intro j hj
               rcases Nat.lt_or_eq_of_le (Nat.lt_succ.mp hj) with hj | hj
-              . apply Or.inr
-                have := hLits j hj
-                simpa using this
+              . exact hEq ▸ hLits j hj
               . apply Or.inl
-                simp [hj])
-      else
-        match unit? with
-        | none =>
-          ⟨τ, .contradiction (by
-            apply le_bot_iff.mp
+                simp [hEq, hj])
+          else
+            ⟨τ, .notUnit⟩
+        | .none =>
+          go (i+1) (some l) (by simp [C.getElem_mem_data hi, hl]) (by
+            intro j hj
+            rcases Nat.lt_or_eq_of_le (Nat.lt_succ.mp hj) with hj | hj
+            . apply Or.inr
+              have := hLits j hj
+              simpa using this
+            . apply Or.inl
+              simp [hj])
+    else
+      match unit? with
+      | none =>
+        ⟨τ, .contradiction (by
+          apply le_bot_iff.mp
+          apply entails_ext.mpr
+          intro σ hσ
+          exfalso
+          rcases (satisfies_conj.mp hσ) with ⟨hσC, hστ⟩
+          have ⟨l, hl, hσl⟩ := Clause.satisfies_iff.mp hσC
+          have ⟨k, hk⟩ := Array.mem_data_iff.mp hl
+          rw [not_lt] at hi
+          have := hLits k (lt_of_lt_of_le k.is_lt hi)
+          simp only [false_or] at this
+          have := entails_ext.mp this _ hστ
+          rw [PropFun.satisfies_neg] at this
+          exact this (hk ▸ hσl))⟩
+      | some u =>
+        ⟨τ.setLit u, .extended u
+          (by simp at hUnit; tauto)
+          (by
+            simp at hUnit
+            simp [τ.toPropFun_setLit_of_none hUnit.right, inf_comm])
+          (by
             apply entails_ext.mpr
             intro σ hσ
-            exfalso
-            rcases (satisfies_conj.mp hσ) with ⟨hσC, hστ⟩
+            have ⟨hστ, hσC⟩ := satisfies_conj.mp hσ
             have ⟨l, hl, hσl⟩ := Clause.satisfies_iff.mp hσC
-            have ⟨k, hk⟩ := Array.mem_data_iff.mp hl
-            rw [not_lt] at hi
-            have := hLits k (lt_of_lt_of_le k.is_lt hi)
-            simp only [false_or] at this
-            have := entails_ext.mp this _ hστ
-            rw [PropFun.satisfies_neg] at this
-            exact this (hk ▸ hσl))⟩
-        | some u =>
-          ⟨τ.setLit u, .extended u
-            (by simp at hUnit; tauto)
-            (by
-              simp at hUnit
-              simp [τ.toPropFun_setLit_of_none u hUnit.right, inf_comm])
-            (by
-              apply entails_ext.mpr
-              intro σ hσ
-              have ⟨hστ, hσC⟩ := satisfies_conj.mp hσ
-              have ⟨l, hl, hσl⟩ := Clause.satisfies_iff.mp hσC
-              have ⟨i, hi⟩ := Array.mem_data_iff.mp hl
-              have := i.is_lt
-              have := hLits i (by linarith)
-              rcases this with hEq | hτl
-              . cases hEq
-                rwa [hi]
-              . exfalso
-                exact (satisfies_neg.mp <| entails_ext.mp hτl _ hστ) (hi ▸ hσl))⟩
-    termination_by go i _ _ _ => C.size - i
+            have ⟨i, hi⟩ := Array.mem_data_iff.mp hl
+            have := i.is_lt
+            have := hLits i (by linarith)
+            rcases this with hEq | hτl
+            . cases hEq
+              rwa [hi]
+            . exfalso
+              exact (satisfies_neg.mp <| entails_ext.mp hτl _ hστ) (hi ▸ hσl))⟩
+  termination_by go i _ _ _ => C.size - i
+
+-- Cayden's alternate implementation of unit propagation (TODO: Compare for efficiency)
+
+section monadic
+
+inductive MUPResult where
+  | falsified
+  | satisfied
+  | unit (l : Ilit) (τ : PPA)    -- Updated assignment and the extending unit literal l
+  | multipleUnassignedLiterals
+
+inductive MUPDone where
+  | satisfied
+  | multipleUnassignedLiterals
+
+open ResultT MUPResult MUPDone
+
+abbrev UPBox := ResultT MUPDone (Option ILit)
+
+def pevalUP (τ : PPA) (unit? : Option ILit) (l : ILit) : UPBox :=
+  match τ.litValue? l with
+  | some true => done .satisfied
+  | some false => ok unit?
+  | none =>
+    match unit? with
+    | none => ok l
+    | some u =>
+      if u = l then ok unit?
+      -- Assume tautology cannot occur in clause, so two unassiged literals exits early
+      else done .multipleUnassignedLiterals
+
+def foldUP (τ : PPA) (C : IClause) := C.foldlM (pevalUP τ) none
+
+def unitProp (τ : PPA) (C : IClause) : MUPResult :=
+  match foldUP τ C with
+  | ok none => .falsified
+  | ok (some lit) => .unit lit (τ.setLit lit)
+  | done .satisfied => .satisfied
+  | done .multipleUnassignedLiterals => .multipleUnassignedLiterals
+
+def motive_fn (τ : PPA) (C : IClause) : ℕ → Option ILit → Prop
+  | idx, none => ∀ ⦃i : Fin C.size⦄, i < idx → τ.litValue? C[i] = some false
+  | idx, some lit => lit ∈ C.data ∧ τ.litValue? lit = none ∧
+      (∀ ⦃j : Fin C.size⦄, j < idx → C[j] ≠ lit → τ.litValue? C[j] = some false)
+
+theorem SatisfiesM_UP (τ : PPA) (C : IClause) :
+    SatisfiesM (fun
+      -- If there are no unassigned literals, then all should be false
+      | none => ∀ l ∈ C.data, τ.litValue? l = some false
+      | some lit => lit ∈ C.data ∧ τ.litValue? lit = none ∧
+          (∀ l ∈ C.data, l ≠ lit → τ.litValue? l = some false)) (foldUP τ C) := by
+  have := C.SatisfiesM_foldlM (init := (none : Option ILit)) (f := pevalUP τ)
+    (motive := motive_fn τ C)
+    (h0 := by simp [motive_fn]) -- Why do I have to define it right above? Putting it inline with (motive :=) had sorryAx problems
+    (hf := by
+      unfold motive_fn
+      simp only [SatisfiesM_ResultT_eq, getElem_fin]
+      intro i box ih
+        -- Cayden question: Is this proof more compact if I use pattern-matching with intro?
+      intro
+      | none, hbox =>
+        simp only
+        intro j hj
+        unfold pevalUP at hbox
+        cases h_tau : τ.litValue? C[i.val] with
+        | none =>
+          simp [h_tau] at hbox
+          cases h_box : box with
+          | none => simp [h_box] at hbox
+          | some lit => by_cases h_lit : lit = C[i.val] <;> simp [h_box, h_lit] at hbox
+        | some b =>
+          cases h_box : box with
+          | none =>
+            subst h_box
+            rcases lt_or_eq_of_le (le_of_lt_succ hj) with (h | h)
+            · exact ih h
+            · cases b
+              · replace h := Fin.ext h; subst h; exact h_tau
+              · simp [h_tau] at hbox
+          | some lit => by_cases h_lit : lit = C[i.val] <;> cases b <;> simp [h_tau, h_box, h_lit] at hbox
+      | some lit, hbox =>
+        unfold pevalUP at hbox
+        cases h_tau : τ.litValue? C[i.val] with
+        | none =>
+          simp [h_tau] at hbox
+          cases h_box : box with
+          | none =>
+            subst h_box
+            simp at hbox
+            use Array.mem_data_iff.mpr ⟨i, hbox⟩, hbox ▸ h_tau
+            intro j hj₁ hj₂
+            rcases lt_or_eq_of_le (le_of_lt_succ hj₁) with (h | h)
+            · exact ih h
+            · simp at ih
+              replace h := Fin.ext h; subst h; rw [hbox] at hj₂; contradiction
+          | some l =>
+            subst h_box
+            by_cases hl : l = C[i.val]
+            · simp [hl] at hbox
+              rw [hbox] at hl
+              subst hl
+              rcases ih with ⟨hl₁, hl₂, ih⟩
+              use hl₁, hl₂
+              intro j hj₁ hj₂
+              rcases lt_or_eq_of_le (le_of_lt_succ hj₁) with (h | h)
+              · exact ih h hj₂
+              · replace h := Fin.ext h; subst h; rw [hbox] at hj₂; contradiction
+            · simp [hl] at hbox
+        | some b =>
+          cases b
+          · simp [h_tau] at hbox
+            subst hbox
+            rcases ih with ⟨hlit₁, hlit₂, ih⟩
+            use hlit₁, hlit₂
+            intro j hj₁ hj₂
+            rcases lt_or_eq_of_le (le_of_lt_succ hj₁) with (h | h)
+            · exact ih h hj₂
+            · replace h := Fin.ext h; subst h; exact h_tau
+          · simp [h_tau] at hbox)
+  apply SatisfiesM.imp this
+  intro
+  | none =>
+    intro h l hl
+    rcases Array.mem_data_iff.mp hl with ⟨i, rfl⟩
+    exact h i.isLt
+  | some lit =>
+    simp [motive_fn]
+    intro hlit₁ hlit₂ ih
+    use hlit₁, hlit₂
+    intro l hl₁ hl₂
+    rcases Array.mem_data_iff.mp hl₁ with ⟨i, rfl⟩
+    exact ih hl₂
+
+-- Cayden TODO/Q: Allow for [pattern_match] on ResultT? What is [unbox]?
+-- Cayden Q: when aesop can't solve something, why does [aesop?] not give anything?
+theorem contradiction_of_UP_falsified {τ : PPA} {C : IClause} :
+    τ.unitProp C = .falsified → τ.toPropFun ⊓ C.toPropFun ≤ ⊥ := by
+  unfold unitProp
+  intro h_falsified
+  split at h_falsified
+  <;> try simp at h_falsified
+  clear h_falsified
+  rename (foldUP τ C = ok none) => h
+  refine entails_ext.mpr fun τ' hτ' => ?_
+  rw [satisfies_conj] at hτ'
+  rcases hτ' with ⟨hττ', hCτ'⟩
+  have ⟨lit, hlit, hτ'lit⟩ := Clause.satisfies_iff.mp hCτ'
+  have hlv := SatisfiesM_ResultT_eq.mp (SatisfiesM_UP τ C) none h lit hlit
+  clear h hCτ' hlit
+  have := satisfies_iff_vars.mp hττ'
+  replace hτ'lit := LitVar.satisfies_iff.mp hτ'lit
+  cases hpol : polarity lit
+  <;> simp [hpol] at hτ'lit
+  <;> simp [litValue?, hpol] at hlv
+  <;> rw [this hlv] at hτ'lit
+  <;> contradiction
+
+-- Is it better to say that ¬(τ ≤ l), or that τ.litValue? l = none?
+theorem extended_of_UP_unit {τ τ' : PPA} {C : IClause} {l : ILit} :
+    τ.unitProp C = .unit l τ' →
+      C.toPropFun ⊓ τ.toPropFun ≤ τ'.toPropFun ∧
+      ¬(τ.toPropFun ≤ l.toPropFun) ∧ (τ'.toPropFun ≤ l.toPropFun) := by
+  unfold unitProp
+  intro h_unit
+  split at h_unit
+  <;> try simp at h_unit
+  rename (ILit) => lit
+  rename (foldUP τ C = ok (some lit)) => h
+  rcases h_unit with ⟨rfl, rfl⟩
+  have hlv := SatisfiesM_ResultT_eq.mp (SatisfiesM_UP τ C) (some lit) h
+  clear h
+  rcases hlv with ⟨hlit, hτlit, h_rest⟩
+  constructor
+  · refine entails_ext.mpr fun τ' hτ' => ?_
+    rw [satisfies_conj] at hτ'; rcases hτ' with ⟨hCτ', hττ'⟩
+    rw [satisfies_iff_lits]; intro l hl
+    by_cases heq : l = lit
+    · subst heq; clear hl
+      rw [Clause.satisfies_iff] at hCτ'; rcases hCτ' with ⟨m, hm, hmτ'⟩
+      by_cases hmeq : m = l
+      · subst hmeq; exact hmτ'
+      · by_cases h_vareq : toVar l = toVar m
+        · have := h_rest _ hm hmeq
+          simp [← negate_eq_of_var_eq_of_ne h_vareq (Ne.symm hmeq), hτlit] at this
+        · rw [satisfies_iff_lits] at hττ'
+          have := litValue?_negate τ m
+          simp only [h_rest _ hm hmeq, Option.map_some', Bool.not_false] at this
+          have := hττ' this
+          simp at this
+          exact absurd hmτ' this
+    · by_cases h_vareq : toVar l = toVar lit
+      · simp [eq_negate_of_var_eq_of_ne h_vareq heq] at hl
+      · rw [litValue?_setLit_of_ne (Ne.symm h_vareq)] at hl
+        exact satisfies_iff_lits.mp hττ' hl
+  · exact ⟨litValue?_none hτlit, litValue?_true (litValue?_setLit τ lit)⟩
+
+end monadic
 
 end PPA
